code/ed25519/Hacl.Impl.Ed25519.Ladder.fst
@@ -95,15 +95,6 @@ let point_double ctx x xx =
 
 
 inline_for_extraction noextract
-let mk_ed25519_concrete_ops : BE.concrete_ops U64 20ul 0ul = {
-  BE.to = mk_to_ed25519_concrete_ops;
-  BE.lmul = point_add;
-  BE.lsqr = point_double;
-}
-
-//////////////////////////////////////////////
-
-inline_for_extraction noextract
 val make_point_inf:
   b:lbuffer uint64 20ul ->
   Stack unit
@@ -125,6 +116,21 @@ let make_point_inf b =
   assert (F51.point_eval h1 b == Spec.Ed25519.point_at_infinity);
   Spec.Ed25519.Lemmas.to_aff_point_at_infinity_lemma ()
 
+
+inline_for_extraction noextract
+val point_zero : BE.lone_st U64 20ul 0ul mk_to_ed25519_concrete_ops
+let point_zero ctx one = make_point_inf one
+
+
+inline_for_extraction noextract
+let mk_ed25519_concrete_ops : BE.concrete_ops U64 20ul 0ul = {
+  BE.to = mk_to_ed25519_concrete_ops;
+  BE.lone = point_zero;
+  BE.lmul = point_add;
+  BE.lsqr = point_double;
+}
+
+//////////////////////////////////////////////
 
 inline_for_extraction noextract
 val make_g:
@@ -157,6 +163,22 @@ let make_g g =
   assert (F51.point_eval h1 g == Spec.Ed25519.g)
 
 
+inline_for_extraction noextract
+val convert_scalar: scalar:lbuffer uint8 32ul -> bscalar:lbuffer uint64 4ul ->
+  Stack unit
+  (requires fun h -> live h scalar /\ live h bscalar /\ disjoint scalar bscalar)
+  (ensures fun h0 _ h1 -> modifies (loc bscalar) h0 h1 /\
+    BD.bn_v h1 bscalar == BSeq.nat_from_bytes_le (as_seq h0 scalar))
+
+let convert_scalar scalar bscalar =
+  let h0 = ST.get () in
+  Lib.ByteBuffer.uints_from_bytes_le bscalar scalar;
+  let h1 = ST.get () in
+  SC.bn_from_bytes_le_is_uints_from_bytes_le #U64 32 (as_seq h0 scalar);
+  assert (as_seq h1 bscalar == SC.bn_from_bytes_le #U64 32 (as_seq h0 scalar));
+  SC.bn_from_bytes_le_lemma #U64 32 (as_seq h0 scalar)
+
+
 val point_mul:
     result:point
   -> scalar:lbuffer uint8 32ul
@@ -175,13 +197,7 @@ let point_mul result scalar q =
   let h0 = ST.get () in
   push_frame ();
   let bscalar = create 4ul (u64 0) in
-  Lib.ByteBuffer.uints_from_bytes_le bscalar scalar;
-  SC.bn_from_bytes_le_is_uints_from_bytes_le #U64 32 (as_seq h0 scalar);
-  let h1 = ST.get () in
-  assert (as_seq h1 bscalar == SC.bn_from_bytes_le #U64 32 (as_seq h0 scalar));
-  SC.bn_from_bytes_le_lemma #U64 32 (as_seq h0 scalar);
-
-  make_point_inf result;
+  convert_scalar scalar bscalar;
   BE.lexp_fw_consttime 20ul 0ul mk_ed25519_concrete_ops (null uint64) q 4ul 256ul bscalar result 4ul;
   pop_frame ()
 
@@ -234,20 +250,11 @@ let point_mul_double_vartime result scalar1 q1 scalar2 q2 =
   let h0 = ST.get () in
   push_frame ();
   let bscalar1 = create 4ul (u64 0) in
-  Lib.ByteBuffer.uints_from_bytes_le bscalar1 scalar1;
-  SC.bn_from_bytes_le_is_uints_from_bytes_le #U64 32 (as_seq h0 scalar1);
-  SC.bn_from_bytes_le_lemma #U64 32 (as_seq h0 scalar1);
+  convert_scalar scalar1 bscalar1;
 
   let bscalar2 = create 4ul (u64 0) in
-  Lib.ByteBuffer.uints_from_bytes_le bscalar2 scalar2;
-  SC.bn_from_bytes_le_is_uints_from_bytes_le #U64 32 (as_seq h0 scalar2);
-  SC.bn_from_bytes_le_lemma #U64 32 (as_seq h0 scalar2);
+  convert_scalar scalar2 bscalar2;
 
-  let h1 = ST.get () in
-  assert (as_seq h1 bscalar1 == SC.bn_from_bytes_le #U64 32 (as_seq h0 scalar1));
-  assert (as_seq h1 bscalar2 == SC.bn_from_bytes_le #U64 32 (as_seq h0 scalar2));
-
-  make_point_inf result;
   ME.lexp_double_fw_vartime 20ul 0ul mk_ed25519_concrete_ops (null uint64) q1 4ul 256ul bscalar1 q2 bscalar2 result 4ul;
   pop_frame ()
 #pop-options
