code/bignum/Hacl.Impl.MultiExponentiation.fsti
@@ -32,30 +32,29 @@ let lexp_double_fw_tables_st
   -> table_len:size_t{1 < v table_len /\ v table_len * v len <= max_size_t /\ v table_len == pow2 (v l)}
   -> table1:lbuffer (uint_t a_t SEC) (table_len *! len)
   -> table2:lbuffer (uint_t a_t SEC) (table_len *! len)
-  -> acc:lbuffer (uint_t a_t SEC) len ->
+  -> res:lbuffer (uint_t a_t SEC) len ->
   Stack unit
   (requires fun h ->
     live h a1 /\ live h b1 /\ live h a2 /\ live h b2 /\
-    live h acc /\ live h ctx /\ live h table1 /\ live h table2 /\
+    live h res /\ live h ctx /\ live h table1 /\ live h table2 /\
 
-    eq_or_disjoint a1 a2 /\ disjoint a1 acc /\ disjoint a1 ctx /\
-    disjoint a1 table1 /\ disjoint a1 table2 /\ disjoint b1 acc /\
-    disjoint a2 acc /\ disjoint a2 ctx /\ disjoint a2 table1 /\ disjoint a2 table2 /\
-    disjoint b2 acc /\ disjoint acc ctx /\ disjoint acc table1 /\ disjoint acc table2 /\
+    eq_or_disjoint a1 a2 /\ disjoint a1 res /\ disjoint a1 ctx /\
+    disjoint a1 table1 /\ disjoint a1 table2 /\ disjoint b1 res /\
+    disjoint a2 res /\ disjoint a2 ctx /\ disjoint a2 table1 /\ disjoint a2 table2 /\
+    disjoint b2 res /\ disjoint res ctx /\ disjoint res table1 /\ disjoint res table2 /\
     disjoint ctx table1 /\ disjoint ctx table2 /\ eq_or_disjoint table1 table2 /\
 
     BD.bn_v h b1 < pow2 (v bBits) /\
     BD.bn_v h b2 < pow2 (v bBits) /\
     k.to.linv_ctx (as_seq h ctx) /\
     k.to.linv (as_seq h a1) /\ k.to.linv (as_seq h a2) /\
-    k.to.linv (as_seq h acc) /\ k.to.refl (as_seq h acc) == k.to.concr_ops.SE.one () /\
     (forall (j:nat{j < v table_len}).
       precomp_table_inv len ctx_len k (as_seq h a1) table_len (as_seq h table1) j) /\
     (forall (j:nat{j < v table_len}).
       precomp_table_inv len ctx_len k (as_seq h a2) table_len (as_seq h table2) j))
-  (ensures  fun h0 _ h1 -> modifies (loc acc) h0 h1 /\
-    k.to.linv (as_seq h1 acc) /\
-    k.to.refl (as_seq h1 acc) ==
+  (ensures  fun h0 _ h1 -> modifies (loc res) h0 h1 /\
+    k.to.linv (as_seq h1 res) /\
+    k.to.refl (as_seq h1 res) ==
     SE.exp_double_fw k.to.concr_ops
       (k.to.refl (as_seq h0 a1)) (v bBits) (BD.bn_v h0 b1)
       (k.to.refl (as_seq h0 a2)) (BD.bn_v h0 b2) (v l))
@@ -102,22 +101,21 @@ let lexp_double_fw_st
   -> b1:lbuffer (uint_t a_t SEC) bLen
   -> a2:lbuffer (uint_t a_t SEC) len
   -> b2:lbuffer (uint_t a_t SEC) bLen
-  -> acc:lbuffer (uint_t a_t SEC) len
+  -> res:lbuffer (uint_t a_t SEC) len
   -> l:size_t{0 < v l /\ v l < bits a_t /\ pow2 (v l) * v len <= max_size_t /\ v l < 32} ->
   Stack unit
   (requires fun h ->
-    live h a1 /\ live h b1 /\ live h a2 /\ live h b2 /\ live h acc /\ live h ctx /\
-    eq_or_disjoint a1 a2 /\ disjoint a1 acc /\ disjoint a1 ctx /\
-    disjoint a2 acc /\ disjoint a2 ctx /\
-    disjoint acc b1 /\ disjoint acc b2 /\ disjoint acc ctx /\
+    live h a1 /\ live h b1 /\ live h a2 /\ live h b2 /\ live h res /\ live h ctx /\
+    eq_or_disjoint a1 a2 /\ disjoint a1 res /\ disjoint a1 ctx /\
+    disjoint a2 res /\ disjoint a2 ctx /\
+    disjoint res b1 /\ disjoint res b2 /\ disjoint res ctx /\
     BD.bn_v h b1 < pow2 (v bBits) /\
     BD.bn_v h b2 < pow2 (v bBits) /\
     k.to.linv_ctx (as_seq h ctx) /\
-    k.to.linv (as_seq h a1) /\ k.to.linv (as_seq h a2) /\
-    k.to.linv (as_seq h acc) /\ k.to.refl (as_seq h acc) == k.to.concr_ops.SE.one ())
-  (ensures  fun h0 _ h1 -> modifies (loc acc) h0 h1 /\
-    k.to.linv (as_seq h1 acc) /\
-    k.to.refl (as_seq h1 acc) ==
+    k.to.linv (as_seq h a1) /\ k.to.linv (as_seq h a2))
+  (ensures  fun h0 _ h1 -> modifies (loc res) h0 h1 /\
+    k.to.linv (as_seq h1 res) /\
+    k.to.refl (as_seq h1 res) ==
     SE.exp_double_fw #k.to.t_spec k.to.concr_ops
       (k.to.refl (as_seq h0 a1)) (v bBits) (BD.bn_v h0 b1)
       (k.to.refl (as_seq h0 a2)) (BD.bn_v h0 b2) (v l))
